ProvabilityLogic/Gentzen/GLAlpha/Basic.lean
@@ -1,0 +1,253 @@
+module
+
+public import ProvabilityLogic.Gentzen.GL.Basic
+public import ProvabilityLogic.Gentzen.GL.WithCut
+
+@[expose]
+public section
+
+open LogicGL
+
+variable {α : Type u} [DecidableEq α]
+
+inductive LogicGLAlpha.ProofGentzen (𝔸 : Set ℕ) : TwoLayeredSequent α → Type u
+| axm (l) (A)      : ProofGentzen 𝔸 ({A} ⟹[l] {A})
+| botL (l)         : ProofGentzen 𝔸 (({⊥} : FormulaFinset α) ⟹[l] ∅)
+| wkL  {l Γ Γ' Δ}  : ProofGentzen 𝔸 (Γ ⟹[l] Δ) → (_ : Γ ⊆ Γ' := by grind) → ProofGentzen 𝔸 (Γ' ⟹[l] Δ)
+| wkR  {l Γ Δ Δ'}  : ProofGentzen 𝔸 (Γ ⟹[l] Δ) → (_ : Δ ⊆ Δ' := by grind) → ProofGentzen 𝔸 (Γ ⟹[l] Δ')
+| impL {l Γ Δ A B} : ProofGentzen 𝔸 (Γ ⟹[l] (insert A Δ)) → ProofGentzen 𝔸 (insert B Γ ⟹[l] Δ) → ProofGentzen 𝔸 ((insert (A 🡒 B) Γ) ⟹[l] Δ)
+| impR {l Γ Δ A B} : ProofGentzen 𝔸 ((insert A Γ) ⟹[l] (insert B Δ)) → ProofGentzen 𝔸 (Γ ⟹[l] (insert (A 🡒 B) Δ))
+| liftUp {Γ Δ}     : ProofGentzen 𝔸 (Γ ⟹[0] Δ) → ProofGentzen 𝔸 (Γ ⟹[1] Δ)
+| boxGL {Γ A}      : ProofGentzen 𝔸 ((insert (□A) (Γ ∪ Γ.box)) ⟹[0] {A}) → ProofGentzen 𝔸 (Γ.box ⟹[0] {□A})
+| boxGP {Γ Δ n}    : n ∈ 𝔸 → ProofGentzen 𝔸 (Γ ⟹[1] insert (□^[n] ⊥) Δ) → ProofGentzen 𝔸 (Γ ⟹[1] Δ)
+
+namespace LogicGLAlpha
+
+scoped notation:120 "⊢ᵍ[GLAlpha " 𝔸 "]! " S => ProofGentzen 𝔸 S
+
+abbrev ProvableGentzen (𝔸 : Set ℕ) (S : TwoLayeredSequent α) : Prop := Nonempty (⊢ᵍ[GLAlpha 𝔸]! S)
+scoped notation:120 "⊢ᵍ[GLAlpha " 𝔸 "] " S => ProvableGentzen 𝔸 S
+
+variable {𝔸 : Set ℕ}
+
+/-- Embed a level-0 `LogicGL` proof into level-0 `LogicGLAlpha`. -/
+def ofProofGentzen {Γ Δ : FormulaFinset α} : ⊢ᵍ[GL]! (Γ ⟹ Δ) → ⊢ᵍ[GLAlpha 𝔸]! (Γ ⟹[0] Δ)
+| .axm A    => .axm 0 A
+| .botL     => .botL 0
+| .wkL h h' => .wkL (ofProofGentzen h) h'
+| .wkR h h' => .wkR (ofProofGentzen h) h'
+| .impL h₁ h₂ => .impL (ofProofGentzen h₁) (ofProofGentzen h₂)
+| .impR h   => .impR (ofProofGentzen h)
+| .boxGL h  => .boxGL (ofProofGentzen h)
+
+/-- Extract a level-0 `LogicGL` proof from level-0 `LogicGLAlpha`. -/
+def toProofGentzen {Γ Δ : FormulaFinset α} : ⊢ᵍ[GLAlpha 𝔸]! (Γ ⟹[0] Δ) → ⊢ᵍ[GL]! (Γ ⟹ Δ)
+| .axm 0 A    => .axm A
+| .botL 0     => .botL
+| .wkL h h'   => .wkL (toProofGentzen h) h'
+| .wkR h h'   => .wkR (toProofGentzen h) h'
+| .impL h₁ h₂ => .impL (toProofGentzen h₁) (toProofGentzen h₂)
+| .impR h     => .impR (toProofGentzen h)
+| .boxGL h    => .boxGL (toProofGentzen h)
+
+/-- Level-`0` `LogicGLAlpha.ProvableGentzen`-provability is exactly (plain, cut-free) `GL`-provability. -/
+theorem iff_provableGentzen_provable_zero {Γ Δ : FormulaFinset α} :
+  (⊢ᵍ[GL] (Γ ⟹ Δ)) ↔ (⊢ᵍ[GLAlpha 𝔸] (Γ ⟹[0] Δ)) :=
+  ⟨λ ⟨h⟩ => ⟨ofProofGentzen h⟩, λ ⟨h⟩ => ⟨toProofGentzen 𝔸 h⟩⟩
+
+namespace ProvableGentzen
+
+variable {𝔸 : Set ℕ}
+variable {Γ Γ' Δ Δ' : FormulaFinset α} {A B : Formula α} {l : Fin 2} {n : ℕ}
+
+lemma axm (l) (A : Formula α) : ⊢ᵍ[GLAlpha 𝔸] ({A} ⟹[l] {A}) := ⟨ProofGentzen.axm l A⟩
+lemma botL (l) : ⊢ᵍ[GLAlpha 𝔸] (({⊥} : FormulaFinset α) ⟹[l] ∅) := ⟨ProofGentzen.botL l⟩
+lemma wkL (π : ⊢ᵍ[GLAlpha 𝔸] (Γ ⟹[l] Δ)) (h : Γ ⊆ Γ') : ⊢ᵍ[GLAlpha 𝔸] (Γ' ⟹[l] Δ) := ⟨ProofGentzen.wkL π.some h⟩
+lemma wkR (π : ⊢ᵍ[GLAlpha 𝔸] (Γ ⟹[l] Δ)) (h : Δ ⊆ Δ') : ⊢ᵍ[GLAlpha 𝔸] (Γ ⟹[l] Δ') := ⟨ProofGentzen.wkR π.some h⟩
+lemma impL (π₁ : ⊢ᵍ[GLAlpha 𝔸] (Γ ⟹[l] insert A Δ)) (π₂ : ⊢ᵍ[GLAlpha 𝔸] (insert B Γ ⟹[l] Δ)) : ⊢ᵍ[GLAlpha 𝔸] ((insert (A 🡒 B) Γ) ⟹[l] Δ) :=
+  ⟨ProofGentzen.impL π₁.some π₂.some⟩
+lemma impR (π : ⊢ᵍ[GLAlpha 𝔸] ((insert A Γ) ⟹[l] (insert B Δ))) : ⊢ᵍ[GLAlpha 𝔸] (Γ ⟹[l] (insert (A 🡒 B) Δ)) := ⟨ProofGentzen.impR π.some⟩
+lemma liftUp (π : ⊢ᵍ[GLAlpha 𝔸] (Γ ⟹[0] Δ)) : ⊢ᵍ[GLAlpha 𝔸] (Γ ⟹[1] Δ) := ⟨ProofGentzen.liftUp π.some⟩
+lemma boxGL (π : ⊢ᵍ[GLAlpha 𝔸] ((insert (□A) (Γ ∪ Γ.box)) ⟹[0] {A})) : ⊢ᵍ[GLAlpha 𝔸] (Γ.box ⟹[0] {□A}) := ⟨ProofGentzen.boxGL π.some⟩
+lemma boxGP (n : n ∈ 𝔸) : ⊢ᵍ[GLAlpha 𝔸] (Γ ⟹[1] insert (□^[n] ⊥) Δ) → ⊢ᵍ[GLAlpha 𝔸] (Γ ⟹[1] Δ) := λ ⟨π⟩ => ⟨ProofGentzen.boxGP π⟩
+
+@[induction_eliminator]
+lemma rec
+  {motive : (S : TwoLayeredSequent α) → ⊢ᵍ[GLAlpha 𝔸] S → Prop}
+  (axm : ∀ (l) (A : Formula α), motive ({A} ⟹[l] {A}) (ProvableGentzen.axm l A))
+  (botL : ∀ (l), motive (({⊥} : FormulaFinset α) ⟹[l] ∅) (ProvableGentzen.botL l))
+  (wkL : ∀ {l Γ Γ' Δ} (π : ⊢ᵍ[GLAlpha 𝔸] (Γ ⟹[l] Δ)) (h : Γ ⊆ Γ'), motive (Γ ⟹[l] Δ) π → motive (Γ' ⟹[l] Δ) (wkL π h))
+  (wkR : ∀ {l Γ Δ Δ'} (π : ⊢ᵍ[GLAlpha 𝔸] (Γ ⟹[l] Δ)) (h : Δ ⊆ Δ'), motive (Γ ⟹[l] Δ) π → motive (Γ ⟹[l] Δ') (wkR π h))
+  (impL : ∀ {l Γ Δ A B} (π₁ : ⊢ᵍ[GLAlpha 𝔸] (Γ ⟹[l] insert A Δ)) (π₂ : ⊢ᵍ[GLAlpha 𝔸] (insert B Γ ⟹[l] Δ)),
+    motive (Γ ⟹[l] insert A Δ) π₁ → motive (insert B Γ ⟹[l] Δ) π₂ →
+    motive ((insert (A 🡒 B) Γ) ⟹[l] Δ) (impL π₁ π₂)
+  )
+  (impR : ∀ {l Γ Δ A B} (π : ⊢ᵍ[GLAlpha 𝔸] ((insert A Γ) ⟹[l] (insert B Δ))),
+    motive ((insert A Γ) ⟹[l] (insert B Δ)) π → motive (Γ ⟹[l] (insert (A 🡒 B) Δ)) (impR π)
+  )
+  (liftUp : ∀ {Γ Δ} (π : ⊢ᵍ[GLAlpha 𝔸] (Γ ⟹[0] Δ)), motive (Γ ⟹[0] Δ) π → motive (Γ ⟹[1] Δ) (liftUp π))
+  (boxGL : ∀ {Γ A} (π : ⊢ᵍ[GLAlpha 𝔸] ((insert (□A) (Γ ∪ Γ.box)) ⟹[0] {A})),
+    motive ((insert (□A) (Γ ∪ Γ.box)) ⟹[0] {A}) π → motive (Γ.box ⟹[0] {□A}) (boxGL π)
+  )
+  (boxGP : ∀ {Γ Δ n} (h : ⊢ᵍ[GLAlpha 𝔸] (Γ ⟹[1] insert (□^[n] ⊥) Δ)),
+    motive (Γ ⟹[1] insert (□^[n] ⊥) Δ) h → motive (Γ ⟹[1] Δ) (boxGP h)
+  )
+  : ∀ {S : TwoLayeredSequent α} (h : ⊢ᵍ[GLAlpha 𝔸] S), motive S h := by
+    rintro S ⟨h⟩;
+    induction h <;> grind;
+
+scoped prefix:120 "⊬ᵍ[GLAlpha 𝔸] " => (¬ ProvableGentzen ·)
+
+lemma iff_unprovableGentzen_isEmpty_ProofGentzen {S : TwoLayeredSequent α} : (⊬ᵍ[GLAlpha 𝔸] S) ↔ (IsEmpty (⊢ᵍ[GLAlpha 𝔸]! S)) := by
+  simp [ProvableGentzen];
+
+/-- Initial sequents with side formulas, at any level. -/
+lemma union (l) (A : Formula α) (hΓ : A ∈ Γ := by grind) (hΔ : A ∈ Δ := by grind) : ⊢ᵍ[GLAlpha 𝔸] (Γ ⟹[l] Δ) :=
+  wkR (wkL (axm l A) (by grind)) (by grind)
+
+lemma union' (l) (A : Formula α) {S : Sequent α} (hΓ : A ∈ S.ant := by grind) (hΔ : A ∈ S.suc := by grind) : ⊢ᵍ[GLAlpha 𝔸] (S.ant ⟹[l] S.suc) :=
+  union l A hΓ hΔ
+
+/-- `botL` with side formulas, at any level. -/
+lemma botL_mem (l) (h : ⊥ ∈ Γ := by grind) : ⊢ᵍ[GLAlpha 𝔸] (Γ ⟹[l] Δ) :=
+  wkR (Δ := ∅) (wkL (botL l) (by grind)) (by grind)
+
+lemma not_provable_zero_of_not_provable_one : ⊬ᵍ[GLAlpha 𝔸] (Γ ⟹[1] Δ) → ⊬ᵍ[GLAlpha 𝔸] (Γ ⟹[0] Δ) := by
+  contrapose!;
+  apply liftUp;
+
+/-- Embed a cut-free `LogicGL` proof of `Γ ⟹ insert (□^[n]⊥) Δ` into level-`1` cut-free
+`LogicGLAlpha` provability of `Γ ⟹[1] Δ`. -/
+lemma of_provableGentzen_insert_boxItr_bot {n : ℕ}
+  (h : ⊢ᵍ[GL] (Γ ⟹ insert (□^[n]⊥) Δ)) : ⊢ᵍ[GLAlpha 𝔸] (Γ ⟹[1] Δ) :=
+  boxGP (liftUp (LogicGLAlpha.iff_provableGentzen_provable_zero.mp h))
+
+end ProvableGentzen
+
+open ProvableGentzen
+
+lemma not_provableGentzen_of_not_provable_one {Γ Δ : FormulaFinset α} (h : ⊬ᵍ[GLAlpha 𝔸] (Γ ⟹[1] Δ)) : ⊬ᵍ[GL] (Γ ⟹ Δ) :=
+  λ hp => ProvableGentzen.not_provable_zero_of_not_provable_one h (iff_provableGentzen_provable_zero.mp hp)
+
+end LogicGLAlpha
+
+
+inductive LogicGLAlpha.GentzenWithCutProof : TwoLayeredSequent α → Type u
+| axm (l) (A)      : GentzenWithCutProof ({A} ⟹[l] {A})
+| botL (l)         : GentzenWithCutProof (({⊥} : FormulaFinset α) ⟹[l] ∅)
+| wkL  {l Γ Γ' Δ}  : GentzenWithCutProof (Γ ⟹[l] Δ) → (_ : Γ ⊆ Γ' := by grind) → GentzenWithCutProof (Γ' ⟹[l] Δ)
+| wkR  {l Γ Δ Δ'}  : GentzenWithCutProof (Γ ⟹[l] Δ) → (_ : Δ ⊆ Δ' := by grind) → GentzenWithCutProof (Γ ⟹[l] Δ')
+| impL {l Γ Δ A B} : GentzenWithCutProof (Γ ⟹[l] (insert A Δ)) → GentzenWithCutProof (insert B Γ ⟹[l] Δ) → GentzenWithCutProof ((insert (A 🡒 B) Γ) ⟹[l] Δ)
+| impR {l Γ Δ A B} : GentzenWithCutProof ((insert A Γ) ⟹[l] (insert B Δ)) → GentzenWithCutProof (Γ ⟹[l] (insert (A 🡒 B) Δ))
+| liftUp {Γ Δ}     : GentzenWithCutProof (Γ ⟹[0] Δ) → GentzenWithCutProof (Γ ⟹[1] Δ)
+| boxGL {Γ A}      : GentzenWithCutProof ((insert (□A) (Γ ∪ Γ.box)) ⟹[0] {A}) → GentzenWithCutProof (Γ.box ⟹[0] {□A})
+| boxGP {Γ Δ n}    : GentzenWithCutProof (Γ ⟹[1] insert (□^[n] ⊥) Δ) → GentzenWithCutProof (Γ ⟹[1] Δ)
+| cut  {l Γ₁ Γ₂ Δ₁ Δ₂ A} : GentzenWithCutProof (Γ₁ ⟹[l] insert A Δ₁) → GentzenWithCutProof (insert A Γ₂ ⟹[l] Δ₂) → GentzenWithCutProof (Γ₁ ∪ Γ₂ ⟹[l] Δ₁ ∪ Δ₂)
+
+namespace LogicGLAlpha
+
+scoped prefix:120 "⊢ᵍᶜ[GLAlpha 𝔸]! " => GentzenWithCutProof
+
+abbrev GentzenWithCutProvable (S : TwoLayeredSequent α) : Prop := Nonempty (⊢ᵍᶜ[GLAlpha 𝔸]! S)
+scoped prefix:120 "⊢ᵍᶜ[GLAlpha 𝔸] " => GentzenWithCutProvable
+
+def GentzenWithCutProof.ofProofGentzen {S : TwoLayeredSequent α} : ⊢ᵍ[GLAlpha 𝔸]! S → ⊢ᵍᶜ[GLAlpha 𝔸]! S
+| .axm l A    => .axm l A
+| .botL l     => .botL l
+| .wkL h h'   => .wkL (GentzenWithCutProof.ofProofGentzen h) h'
+| .wkR h h'   => .wkR (GentzenWithCutProof.ofProofGentzen h) h'
+| .impL h₁ h₂ => .impL (GentzenWithCutProof.ofProofGentzen h₁) (GentzenWithCutProof.ofProofGentzen h₂)
+| .impR h     => .impR (GentzenWithCutProof.ofProofGentzen h)
+| .liftUp h   => .liftUp (GentzenWithCutProof.ofProofGentzen h)
+| .boxGL h    => .boxGL (GentzenWithCutProof.ofProofGentzen h)
+| .boxGP h    => .boxGP (GentzenWithCutProof.ofProofGentzen h)
+
+def GentzenWithCutProof.toGentzenWithCutProofGL {Γ Δ : FormulaFinset α} : ⊢ᵍᶜ[GLAlpha 𝔸]! (Γ ⟹[0] Δ) → ⊢ᵍᶜ[GL]! (Γ ⟹ Δ)
+| .axm 0 A    => .axm A
+| .botL 0     => .botL
+| .wkL h h'   => .wkL (GentzenWithCutProof.toGentzenWithCutProofGL h) h'
+| .wkR h h'   => .wkR (GentzenWithCutProof.toGentzenWithCutProofGL h) h'
+| .impL h₁ h₂ => .impL (GentzenWithCutProof.toGentzenWithCutProofGL h₁) (GentzenWithCutProof.toGentzenWithCutProofGL h₂)
+| .impR h     => .impR (GentzenWithCutProof.toGentzenWithCutProofGL h)
+| .boxGL h    => .boxGL (GentzenWithCutProof.toGentzenWithCutProofGL h)
+| .cut h₁ h₂  => .cut (GentzenWithCutProof.toGentzenWithCutProofGL h₁) (GentzenWithCutProof.toGentzenWithCutProofGL h₂)
+
+namespace GentzenWithCutProvable
+
+variable {S : TwoLayeredSequent α} {Γ Γ' Δ Δ' Γ₁ Γ₂ Δ₁ Δ₂ : FormulaFinset α} {A B : Formula α} {l : Fin 2}
+
+theorem of_without_cut : ⊢ᵍ[GLAlpha 𝔸] S → ⊢ᵍᶜ[GLAlpha 𝔸] S := λ ⟨h⟩ => ⟨GentzenWithCutProof.ofProofGentzen h⟩
+
+/-- `Prop`-level version of `LogicGLAlpha.GentzenWithCutProof.toGentzenWithCutProofGL`. -/
+theorem toGentzenWithCutProvableGL {Γ Δ : FormulaFinset α} (h : ⊢ᵍᶜ[GLAlpha 𝔸] (Γ ⟹[0] Δ)) : ⊢ᵍᶜ[GL] (Γ ⟹ Δ) :=
+  ⟨GentzenWithCutProof.toGentzenWithCutProofGL h.some⟩
+
+/-- Level-`0` `LogicGLAlpha`-with-cut provability implies cut-free `LogicGL`-Gentzen provability. -/
+theorem toProvableGentzenGL {Γ Δ : FormulaFinset α} (h : ⊢ᵍᶜ[GLAlpha 𝔸] (Γ ⟹[0] Δ)) : ⊢ᵍ[GL] (Γ ⟹ Δ) :=
+  LogicGL.ProvableGentzen.of_with_cut (toGentzenWithCutProvableGL h)
+
+lemma axm (l) (A : Formula α) : ⊢ᵍᶜ[GLAlpha 𝔸] ({A} ⟹[l] {A}) := ⟨GentzenWithCutProof.axm l A⟩
+lemma botL (l) : ⊢ᵍᶜ[GLAlpha 𝔸] (({⊥} : FormulaFinset α) ⟹[l] ∅) := ⟨GentzenWithCutProof.botL l⟩
+lemma wkL (h : ⊢ᵍᶜ[GLAlpha 𝔸] (Γ ⟹[l] Δ)) (h' : Γ ⊆ Γ') : ⊢ᵍᶜ[GLAlpha 𝔸] (Γ' ⟹[l] Δ) := ⟨GentzenWithCutProof.wkL h.some h'⟩
+lemma wkR (h : ⊢ᵍᶜ[GLAlpha 𝔸] (Γ ⟹[l] Δ)) (h' : Δ ⊆ Δ') : ⊢ᵍᶜ[GLAlpha 𝔸] (Γ ⟹[l] Δ') := ⟨GentzenWithCutProof.wkR h.some h'⟩
+lemma impL (h₁ : ⊢ᵍᶜ[GLAlpha 𝔸] (Γ ⟹[l] insert A Δ)) (h₂ : ⊢ᵍᶜ[GLAlpha 𝔸] (insert B Γ ⟹[l] Δ)) : ⊢ᵍᶜ[GLAlpha 𝔸] ((insert (A 🡒 B) Γ) ⟹[l] Δ) :=
+  ⟨GentzenWithCutProof.impL h₁.some h₂.some⟩
+lemma impR (h : ⊢ᵍᶜ[GLAlpha 𝔸] ((insert A Γ) ⟹[l] (insert B Δ))) : ⊢ᵍᶜ[GLAlpha 𝔸] (Γ ⟹[l] (insert (A 🡒 B) Δ)) := ⟨GentzenWithCutProof.impR h.some⟩
+lemma liftUp (h : ⊢ᵍᶜ[GLAlpha 𝔸] (Γ ⟹[0] Δ)) : ⊢ᵍᶜ[GLAlpha 𝔸] (Γ ⟹[1] Δ) := ⟨GentzenWithCutProof.liftUp h.some⟩
+lemma boxGL (h : ⊢ᵍᶜ[GLAlpha 𝔸] ((insert (□A) (Γ ∪ Γ.box)) ⟹[0] {A})) : ⊢ᵍᶜ[GLAlpha 𝔸] (Γ.box ⟹[0] {□A}) := ⟨GentzenWithCutProof.boxGL h.some⟩
+lemma boxGP (h : ⊢ᵍᶜ[GLAlpha 𝔸] (Γ ⟹[1] insert (□^[n] ⊥) Δ)) : ⊢ᵍᶜ[GLAlpha 𝔸] (Γ ⟹[1] Δ) := ⟨GentzenWithCutProof.boxGP h.some⟩
+lemma cut (h₁ : ⊢ᵍᶜ[GLAlpha 𝔸] (Γ₁ ⟹[l] insert A Δ₁)) (h₂ : ⊢ᵍᶜ[GLAlpha 𝔸] (insert A Γ₂ ⟹[l] Δ₂)) : ⊢ᵍᶜ[GLAlpha 𝔸] (Γ₁ ∪ Γ₂ ⟹[l] Δ₁ ∪ Δ₂) :=
+  ⟨GentzenWithCutProof.cut h₁.some h₂.some⟩
+
+@[induction_eliminator]
+lemma rec
+  {motive : (S : TwoLayeredSequent α) → ⊢ᵍᶜ[GLAlpha 𝔸] S → Prop}
+  (axm : ∀ (l) (A : Formula α), motive ({A} ⟹[l] {A}) (GentzenWithCutProvable.axm l A))
+  (botL : ∀ (l), motive (({⊥} : FormulaFinset α) ⟹[l] ∅) (GentzenWithCutProvable.botL l))
+  (wkL : ∀ {l Γ Γ' Δ} (h : ⊢ᵍᶜ[GLAlpha 𝔸] (Γ ⟹[l] Δ)) (h' : Γ ⊆ Γ'), motive (Γ ⟹[l] Δ) h → motive (Γ' ⟹[l] Δ) (wkL h h'))
+  (wkR : ∀ {l Γ Δ Δ'} (h : ⊢ᵍᶜ[GLAlpha 𝔸] (Γ ⟹[l] Δ)) (h' : Δ ⊆ Δ'), motive (Γ ⟹[l] Δ) h → motive (Γ ⟹[l] Δ') (wkR h h'))
+  (impL : ∀ {l Γ Δ A B} (h₁ : ⊢ᵍᶜ[GLAlpha 𝔸] (Γ ⟹[l] insert A Δ)) (h₂ : ⊢ᵍᶜ[GLAlpha 𝔸] (insert B Γ ⟹[l] Δ)),
+    motive (Γ ⟹[l] insert A Δ) h₁ → motive (insert B Γ ⟹[l] Δ) h₂ →
+    motive ((insert (A 🡒 B) Γ) ⟹[l] Δ) (impL h₁ h₂)
+  )
+  (impR : ∀ {l Γ Δ A B} (h : ⊢ᵍᶜ[GLAlpha 𝔸] ((insert A Γ) ⟹[l] (insert B Δ))),
+    motive ((insert A Γ) ⟹[l] (insert B Δ)) h → motive (Γ ⟹[l] (insert (A 🡒 B) Δ)) (impR h)
+  )
+  (liftUp : ∀ {Γ Δ} (h : ⊢ᵍᶜ[GLAlpha 𝔸] (Γ ⟹[0] Δ)), motive (Γ ⟹[0] Δ) h → motive (Γ ⟹[1] Δ) (liftUp h))
+  (boxGL : ∀ {Γ A} (h : ⊢ᵍᶜ[GLAlpha 𝔸] ((insert (□A) (Γ ∪ Γ.box)) ⟹[0] {A})),
+    motive ((insert (□A) (Γ ∪ Γ.box)) ⟹[0] {A}) h → motive (Γ.box ⟹[0] {□A}) (boxGL h)
+  )
+  (boxGP : ∀ {Γ Δ n} (h : ⊢ᵍᶜ[GLAlpha 𝔸] (Γ ⟹[1] insert (□^[n] ⊥) Δ)),
+    motive (Γ ⟹[1] insert (□^[n] ⊥) Δ) h → motive (Γ ⟹[1] Δ) (boxGP h)
+  )
+  (cut : ∀ {l Γ₁ Γ₂ Δ₁ Δ₂ A} (h₁ : ⊢ᵍᶜ[GLAlpha 𝔸] (Γ₁ ⟹[l] insert A Δ₁)) (h₂ : ⊢ᵍᶜ[GLAlpha 𝔸] (insert A Γ₂ ⟹[l] Δ₂)),
+    motive (Γ₁ ⟹[l] insert A Δ₁) h₁ → motive (insert A Γ₂ ⟹[l] Δ₂) h₂ →
+    motive (Γ₁ ∪ Γ₂ ⟹[l] Δ₁ ∪ Δ₂) (GentzenWithCutProvable.cut h₁ h₂)
+  )
+  : ∀ {S : TwoLayeredSequent α} (h : ⊢ᵍᶜ[GLAlpha 𝔸] S), motive S h := by
+    rintro S ⟨h⟩;
+    induction h <;> grind;
+
+/-- The axiom `∼□^[n]⊥` is with-cut-provable at level `1`. -/
+lemma neg_boxItr_bot (n : ℕ) : ⊢ᵍᶜ[GLAlpha 𝔸] ((∅ : FormulaFinset α) ⟹[1] {∼□^[n]⊥}) := by
+  show ⊢ᵍᶜ[GLAlpha 𝔸] ((∅ : FormulaFinset α) ⟹[1] {□^[n]⊥ 🡒 ⊥});
+  rw [← Finset.insert_empty];
+  apply impR;
+  apply boxGP (n := n);
+  apply wkR (axm 1 (□^[n]⊥));
+  grind;
+
+/-- Modus ponens for level-`1` with-cut provability, via the `cut` rule. -/
+lemma mdp (hAB : ⊢ᵍᶜ[GLAlpha 𝔸] (∅ ⟹[1] {A 🡒 B})) (hA : ⊢ᵍᶜ[GLAlpha 𝔸] (∅ ⟹[1] {A})) : ⊢ᵍᶜ[GLAlpha 𝔸] (∅ ⟹[1] {B}) := by
+  have h₁ : ⊢ᵍᶜ[GLAlpha 𝔸] ((insert (A 🡒 B) (∅ : FormulaFinset α)) ⟹[1] {B}) :=
+    impL (wkR hA (by grind)) (wkL (axm 1 B) (by grind));
+  have h₂ : ⊢ᵍᶜ[GLAlpha 𝔸] ((∅ : FormulaFinset α) ⟹[1] insert (A 🡒 B) (∅ : FormulaFinset α)) := by
+    rwa [Finset.insert_empty];
+  simpa using cut h₂ h₁;
+
+end GentzenWithCutProvable
+
+end LogicGLAlpha
+
+
+end
