ProvabilityLogic/Logic/GLAlpha/Basic.lean
@@ -1,0 +1,15 @@
+module
+
+public import ProvabilityLogic.Logic.GL.Letterless
+public import ProvabilityLogic.Kripke.FiniteLineModel
+public import ProvabilityLogic.ToFoundation.Vorspiel.Set.Basic
+public import ProvabilityLogic.Formula.Countable
+public import ProvabilityLogic.ProvabilityLogic.GL.Uniform
+public import ProvabilityLogic.ToFoundation.FirstOrder.Basic.Compactness
+
+@[expose]
+public section
+
+abbrev LogicGLAlpha {α} (𝔸 : Set ℕ) : Logic α := (@LogicGL α) +ᴸ ↑(𝔸.image $ TBB (α := Empty))
+
+end
